TaPL/code/chapter3_error.v
@@ -1,0 +1,103 @@
+Require Import Psatz.
+Require Import Classical.
+
+
+Inductive term : Type :=
+  | True: term
+  | False: term
+  | If: term -> term-> term-> term
+  | O: term
+  | Succ: term -> term
+  | Pred: term -> term
+  | Iszero: term -> term
+  | Wrong: term.
+
+Inductive nvalue: term -> Prop :=
+| nv_zero: nvalue O
+| nv_succ: forall nv, nvalue nv -> nvalue (Succ nv).
+
+Inductive value: term -> Prop :=
+| v_true: value True
+| v_false: value False
+| v_nv: forall nv, nvalue nv -> value nv
+| v_wrong: value Wrong.
+
+Inductive badnat: term -> Prop :=
+| bn_wrong: badnat Wrong
+| bn_true: badnat True
+| bn_false: badnat False.
+
+Inductive badbool: term -> Prop :=
+| bb_wrong: badbool Wrong
+| bb_nv: forall nv, nvalue nv -> badbool nv.
+
+Inductive NoWrong: term -> Prop :=
+| nw_true: NoWrong True
+| nw_false: NoWrong False
+| nw_O: NoWrong O
+| nw_succ: forall t, NoWrong t -> NoWrong (Succ t)
+| nw_pred: forall t, NoWrong t -> NoWrong (Pred t)
+| nw_iszero: forall t, NoWrong t -> NoWrong (Iszero t) 
+| nw_if: forall t1 t2 t3, NoWrong t1 -> NoWrong t2 -> NoWrong t3 -> NoWrong (If t1 t2 t3).
+
+Inductive step: term -> term-> Prop :=
+  | EIfTrue: forall t2 t3, step (If True t2 t3) t2
+  | EIfFalse: forall t2 t3, step (If False t2 t3) t3
+  | EIf: forall t1 t1' t2 t3, (step t1 t1') -> (step (If t1 t2 t3) (If t1' t2 t3))
+  | ESucc: forall t1 t1', step t1 t1' -> step (Succ t1) (Succ t1')
+  | EPredZero: step (Pred O) O
+  | EPredSucc: forall nv, step (Pred (Succ nv)) nv
+  | EPred: forall t1 t1', step t1 t1' -> step (Pred t1) (Pred t1')
+  | EIsZeroZero: step (Iszero O) True
+  | EIsZeroSucc: forall nv, step (Iszero (Succ nv)) False
+  | EIsZero: forall t1 t1', step t1 t1' -> step (Iszero t1) (Iszero t1')
+
+  | EIfWrong: forall t1 t2 t3, badbool t1 -> step (If t1 t2 t3) Wrong
+  | ESuccWrong: forall t, badnat t -> step (Succ t) Wrong
+  | EPredWrong: forall t, badnat t -> step (Pred t) Wrong
+  | EIsZeroWrong: forall t, badnat t -> step (Iszero t) Wrong.
+
+Inductive goodstep: term -> term -> Prop :=
+  | EGood: forall t1 t2, NoWrong t1 -> NoWrong t2 -> step t1 t2 -> goodstep t1 t2.
+
+Lemma wrongnogood:  not (NoWrong Wrong). unfold not. intros. inversion H. Qed.
+
+Definition relation (X : Type) := X -> X -> Prop.
+
+Inductive multistep: term -> term -> Prop :=
+| Refl: forall t, multistep t t
+| Trans: forall t1 t2 t3, step t1 t2 -> multistep t2 t3 -> multistep t1 t3.
+
+Inductive multigoodstep: term -> term -> Prop :=
+| EMultiGood: forall t, NoWrong t -> multigoodstep t t
+| ETransGood: forall t1 t2 t3, goodstep t1 t2 -> multigoodstep t2 t3 -> multigoodstep t1 t3.
+
+Inductive normalstop: term -> Prop :=
+| nexist: forall t, NoWrong t -> (forall t1, not (goodstep t t1)) -> not (value t) -> normalstop t.
+
+Lemma nowrongnv: forall nv, nvalue nv -> NoWrong nv.
+intros. induction H. apply nw_O. apply nw_succ. apply IHnvalue. Qed.
+
+Lemma nvstep: forall nv t, nvalue nv -> not (step nv t). unfold not.
+intros. generalize dependent t. induction H. intros. inversion H0. intros.
+inversion H0. subst. apply IHnvalue in H2.  auto. subst. inversion H2. subst.
+inversion H. subst. inversion H. subst. inversion H. Qed.
+
+Lemma thm3_5_4: forall t t1 t2, step t t1 -> step t t2 -> t1 = t2. Admitted.
+
+(* Lemma multistepexistsvalue: forall t, exists v, multistep t v /\ value v. Admitted. *)
+
+Lemma A4: forall t, normalstop t -> multistep t Wrong.
+intros. Admitted.
+
+Theorem thm3_5_16: forall t, NoWrong t -> ((exists u, multigoodstep t u /\ normalstop u) <-> (exists v, multistep t v /\ v = Wrong)).
+intros. split. intros. destruct H0. destruct H0. induction H0.
+apply A4 in H1. exists Wrong. split. apply H1. reflexivity. inversion H0. apply IHmultigoodstep in H4. destruct H4. destruct H4.
+exists x. split. inversion H0. apply Trans with (t2:=t2). apply H5. apply H4. apply H8. apply H1.
+intros. destruct H0. destruct H0. induction H0.
+subst. inversion H. assert ((goodstep t1 t2) \/ not (goodstep t1 t2)). apply classic. destruct H3.
+inversion H3. apply IHmultistep in H5. destruct H5. destruct H5. exists x. split. apply ETransGood with t2.
+apply H3. apply H5. apply H9. apply H1. exists t1. split. apply EMultiGood. apply H. apply nexist.
+apply H. unfold not. intros. assert (t0 = t2). inversion H4. apply thm3_5_4 with t1. apply H7. apply H0.
+subst. contradiction. unfold not. intros. destruct H4. inversion H0. inversion H0. apply nvstep with (nv:=nv) (t:=t2) in H0.
+apply H0. apply H4. inversion H0. Qed.
